thy/Rot13.thy
@@ -34,7 +34,10 @@ definition "rot13 =  ''
 
 
 (*the exprected value of rev ''Uryyb Jbeyq'' = ''qyebJ byyrU'' can be seen*)
-value[code] "run_bf (parse_instrs rot13) (''Hello World''::char list)"
+value[code] "(map char_to_byte ''Hello World'')"
+value[code] "(parse_instrs rot13)"
+value[code] "run_bf (parse_instrs rot13) (map char_to_byte ''Hello World'')"
+value[code] "let v = run_bf (parse_instrs rot13) (''Hello World''::char list) in ()"
 (*todo: present output somehow, even if program wants to continue processing input*)
 
 end
